src/coq/Memory.v
@@ -34,10 +34,6 @@ Definition mem_step {X} (e:effects X) (m:memory) :=
 
   | Call _ _ _ => inl e
   end.
-Print mem_step.
-Print instr.
-Print effects.
-
 
 CoFixpoint memD (m:memory) (d:Trace ()) : Trace () :=
   match d with
